Add a bunch of documentation
This also renames gen_heap to heap_map, since it's no longer general.

src/heap_lib.v
@@ -4,7 +4,9 @@ From iris.proofmode Require Import tactics.
 From iris_simp_lang Require Import heap_ra.
 From iris.prelude Require Import options.
 
-(** This file is a "ghost state" library on top of heap_ra.
+(*|
+
+This file is a "ghost state" library on top of heap_ra.
 
 It defines Iris propositions for owning the ghost state that will track the
 simp_lang heap and the points-to facts that will give the right to read and write
@@ -14,43 +16,43 @@ easier to use, since it is now stated in terms of updates in the Iris logic
 rather than theorems about the RA (so for example these theorems can be used
 directly in the IPM).
 
-*)
+|*)
 
-Class gen_heapGpreS (L V : Type) (Σ : gFunctors) `{Countable L} := {
-  gen_heapGpreS_inG :> inG Σ (heap_mapR L V);
+Class heap_mapGpreS (L V : Type) (Σ : gFunctors) `{Countable L} := {
+  heap_mapGpreS_inG :> inG Σ (heap_mapR L V);
 }.
 
-Class gen_heapGS (L V : Type) (Σ : gFunctors) `{Countable L} := GenHeapGS {
-  gen_heap_inG :> gen_heapGpreS L V Σ;
-  gen_heap_name : gname;
+Class heap_mapGS (L V : Type) (Σ : gFunctors) `{Countable L} := GenHeapGS {
+  heap_map_inG :> heap_mapGpreS L V Σ;
+  heap_map_name : gname;
 }.
 Global Arguments GenHeapGS L V Σ {_ _ _} _ : assert.
-Global Arguments gen_heap_name {L V Σ _ _} _ : assert.
+Global Arguments heap_map_name {L V Σ _ _} _ : assert.
 
-Definition gen_heapΣ (L V : Type) `{Countable L} : gFunctors := #[
+Definition heap_mapΣ (L V : Type) `{Countable L} : gFunctors := #[
   GFunctor (heap_mapR L V)
 ].
 
-Global Instance subG_gen_heapGpreS {Σ L V} `{Countable L} :
-  subG (gen_heapΣ L V) Σ → gen_heapGpreS L V Σ.
+Global Instance subG_heap_mapGpreS {Σ L V} `{Countable L} :
+  subG (heap_mapΣ L V) Σ → heap_mapGpreS L V Σ.
 Proof. solve_inG. Qed.
 
 Section definitions.
-  Context `{Countable L, hG : !gen_heapGS L V Σ}.
+  Context `{Countable L, hG : !heap_mapGS L V Σ}.
 
   (*|
   These two definitions are the key idea behind the state interpretation.
-  `gen_heap_interp` is the authoritative element of this RA, which will be the
+  `heap_map_interp` is the authoritative element of this RA, which will be the
   state interpretation of `σ`, while `mapsto_def` has fragments that live outside
   the state interpretation and are owned by threads. `l ↦ v` will be notation for
   `mapsto`, with a full 1 fraction.
   |*)
 
-    Definition gen_heap_interp (σ : gmap L V) : iProp Σ :=
-      own (gen_heap_name hG) (Auth (σ : gmap L V)).
+    Definition heap_map_interp (σ : gmap L V) : iProp Σ :=
+      own (heap_map_name hG) (Auth (σ : gmap L V)).
 
     Definition mapsto_def (l : L) (v: V) : iProp Σ :=
-      own (gen_heap_name hG) (Frag {[l := v]}).
+      own (heap_map_name hG) (Frag {[l := v]}).
     Definition mapsto_aux : seal (@mapsto_def). Proof. by eexists. Qed.
     Definition mapsto := mapsto_aux.(unseal).
     Definition mapsto_eq : @mapsto = @mapsto_def := mapsto_aux.(seal_eq).
@@ -59,8 +61,8 @@ End definitions.
 Notation "l ↦ v" := (mapsto l v)
   (at level 20, format "l  ↦  v") : bi_scope.
 
-Section gen_heap.
-  Context {L V} `{Countable L, !gen_heapGS L V Σ}.
+Section heap_map.
+  Context {L V} `{Countable L, !heap_mapGS L V Σ}.
   Implicit Types (P Q : iProp Σ).
   Implicit Types (Φ : V → iProp Σ).
   Implicit Types (σ : gmap L V) (l : L) (v : V).
@@ -78,37 +80,37 @@ Section gen_heap.
   Qed.
 
   (** Update lemmas *)
-  Lemma gen_heap_alloc σ l v :
+  Lemma heap_map_alloc σ l v :
     σ !! l = None →
-    gen_heap_interp σ ==∗ gen_heap_interp (<[l:=v]>σ) ∗ l ↦ v.
+    heap_map_interp σ ==∗ heap_map_interp (<[l:=v]>σ) ∗ l ↦ v.
   Proof.
-    iIntros (Hσl). rewrite /gen_heap_interp mapsto_eq /mapsto_def /=.
+    iIntros (Hσl). rewrite /heap_map_interp mapsto_eq /mapsto_def /=.
     iIntros "Hσ".
     iMod (own_update with "Hσ") as "[Hσ Hl]".
     { eapply (heap_map_alloc_update _ l); done. }
     iModIntro. iFrame.
   Qed.
 
-  Lemma gen_heap_valid σ l v : gen_heap_interp σ -∗ l ↦ v -∗ ⌜σ !! l = Some v⌝.
+  Lemma heap_map_valid σ l v : heap_map_interp σ -∗ l ↦ v -∗ ⌜σ !! l = Some v⌝.
   Proof.
     iIntros "Hσ Hl".
-    rewrite /gen_heap_interp mapsto_eq.
+    rewrite /heap_map_interp mapsto_eq /mapsto_def.
     by iDestruct (own_valid_2 with "Hσ Hl") as %Hsub%heap_map_singleton_valid.
   Qed.
 
-  Lemma gen_heap_update σ l v1 v2 :
-    gen_heap_interp σ -∗ l ↦ v1 ==∗ gen_heap_interp (<[l:=v2]>σ) ∗ l ↦ v2.
+  Lemma heap_map_update σ l v1 v2 :
+    heap_map_interp σ -∗ l ↦ v1 ==∗ heap_map_interp (<[l:=v2]>σ) ∗ l ↦ v2.
   Proof.
     iIntros "Hσ Hl".
-    rewrite /gen_heap_interp mapsto_eq /mapsto_def.
+    rewrite /heap_map_interp mapsto_eq /mapsto_def.
     iMod (own_update_2 with "Hσ Hl") as "[Hσ Hl]".
     { eapply heap_map_modify_update. }
     iModIntro. iFrame.
   Qed.
-End gen_heap.
+End heap_map.
 
-Lemma gen_heap_init `{Countable L, !gen_heapGpreS L V Σ} σ :
-  ⊢ |==> ∃ _ : gen_heapGS L V Σ, gen_heap_interp σ.
+Lemma heap_map_init `{Countable L, !heap_mapGpreS L V Σ} σ :
+  ⊢ |==> ∃ _ : heap_mapGS L V Σ, heap_map_interp σ.
 Proof.
   iMod (own_alloc (Auth (σ : gmap L V))) as (γ) "Hσ".
   { exact: heap_map_auth_valid.  }
